coq/LLVMGen/Correctness_NExpr.v
@@ -97,21 +97,265 @@ Section NExpr.
 
   Ltac split_post := split; [split | split]; [solve_state_invariant | solve_fresh | | cbn; intuition].
 
-  Lemma genNExpr_correct_ind :
+  (* Variant precond σ (s1 s2 : IRState) (l_i : local_env): memoryH -> config_cfg -> Prop := *)
+  (* | build_precond : forall mH mV l g *)
+  (*                     (MINV: memory_invariant σ s1 mH (mV,(l_i,g))) *)
+  (*                     (WF: WF_IRState σ s1) *)
+  (*                     (FRESH: freshness s1 s2 l_i l), *)
+  (*     precond σ s1 s2 l_i mH (mV,(l,g)). *)
+ 
+  (* Variant postcond σ (s1 s2 : IRState) (l_i : local_env): memoryH -> config_cfg -> Prop := *)
+  (* | build_postcond : forall mH mV l g *)
+  (*                     (MINV: memory_invariant σ s2 mH (mV,(l_i,g))) *)
+  (*                     (WF: WF_IRState σ s2) *)
+  (*                     (FRESH: freshness s1 s2 l_i l), *)
+  (*     postcond σ s1 s2 l_i mH (mV,(l,g)). *)
+
+
+  Lemma state_invariant_sub_alist:
+    forall σ s mH mV l1 l2 g,
+      l1 ⊑ l2 ->
+      state_invariant σ s mH (mV,(l1,g)) ->
+      state_invariant σ s mH (mV,(l2,g)). 
+  Proof.
+    intros * SUB [MEM WF].
+    split; auto.
+    cbn; intros * LUH LUV.
+    eapply MEM in LUH; eapply LUH in LUV; clear MEM LUH.
+    destruct v, x; cbn in *; auto.
+    - apply SUB in LUV; auto.
+    - apply SUB in LUV; auto.
+    - destruct LUV as (? & ? & ? & LU & ?); do 2 eexists; repeat split; eauto.
+      apply SUB in LU; auto.
+  Qed.
+
+  Lemma freshness_ext : forall s1 s2 l1 l2,
+      extends s1 s2 l1 l2 ->
+      l1 ⊑ l2.
+  Proof.
+    intros * FRESH; apply FRESH.
+  Qed.
+
+  Lemma state_invariant_memory_invariant :
+    forall σ s1 s2 s li mH mV l g,
+      state_invariant' σ s1 s2 s li mH (mV,(l,g)) ->
+      memory_invariant σ s mH (mV,(li,g)).
+  Proof.
+    intros * H; inv H; auto.
+  Qed.
+  Hint Resolve state_invariant_memory_invariant : core.
+  Import LidBound.
+
+  Lemma sub_alist_add' :
+    forall {K V : Type} {RD:RelDec (@Logic.eq K)} {RDC:RelDec_Correct RD} k v (m1 m2 : alist K V),
+      alist_fresh k m1 ->
+      m1 ⊑ m2 ->
+      m1 ⊑ (alist_add k v m2).
+  Proof.
+    repeat intro.
+    unfold alist_In, alist_fresh in *.
+    destruct (rel_dec_p k id).
+    - subst; rewrite H in H1; inversion H1.
+    - apply In_In_add_ineq; auto.
+  Qed.
+
+
+
+  Lemma state_invariant_add_fresh' :
+    ∀ (σ : evalContext) (s1 s2 : IRState) (id : raw_id) (memH : memoryH) (memV : memoryV) 
+      (li l : local_env) (g : global_env) (v : uvalue),
+      incLocal s1 ≡ inr (s2, id)
+      → state_invariant' σ s1 s2 s1 li memH (memV, (l, g))
+      → state_invariant' σ s1 s2 s2 li memH (memV, (alist_add id v l, g)).
+  Proof.
+    intros * INC INV; inv INV.
+    constructor.
+    - red; intros * LUH LUV.
+      erewrite incLocal_Γ in LUV; eauto.
+      generalize LUV; intros INLG;
+        eapply MINV in INLG; eauto.
+    - unfold WF_IRState; erewrite incLocal_Γ; eauto; apply WF.
+    - destruct EXT as [EXT DOM].
+      split.
+      + apply sub_alist_add'; auto.
+        eapply is_fresh_alist_fresh; eauto.
+      + intros * IN NIN.
+        destruct (id ?[ Logic.eq ] id0) eqn:EQ.
+        * rewrite rel_dec_correct in EQ; subst; auto using lid_bound_between_incLocal.
+        * apply neg_rel_dec_correct in EQ.
+          apply In_add_In_ineq in IN; eauto.
+    - solve_fresh.
+  Qed.
+
+  Variant state_invariant'' (σ : evalContext) (s1 s2 s : IRState) (li: local_env): memoryH -> config_cfg -> Prop :=
+  | mk_state_invariant' : forall mH mV l g
+                            (MINV : memory_invariant σ s mH (mV, (li, g)))
+                            (WF   : WF_IRState σ s)
+                            (EXT  : li ⊑ l)
+                            (FRESH: is_fresh s1 s2 li),
+      state_invariant'' σ s1 s2 s li mH (mV,(l,g)).
+
+
+  Lemma state_invariant_add_fresh'' :
+    ∀ (σ : evalContext) (s1 s2 : IRState) (id : raw_id) (memH : memoryH) (memV : memoryV) 
+      (li l : local_env) (g : global_env) (v : uvalue),
+      incLocal s1 ≡ inr (s2, id)
+      → state_invariant'' σ s1 s2 s1 li memH (memV, (l, g))
+      → state_invariant'' σ s1 s2 s2 li memH (memV, (alist_add id v l, g)).
+  Proof.
+    intros * INC INV; inv INV.
+    constructor.
+    - red; intros * LUH LUV.
+      erewrite incLocal_Γ in LUV; eauto.
+      generalize LUV; intros INLG;
+        eapply MINV in INLG; eauto.
+    - unfold WF_IRState; erewrite incLocal_Γ; eauto; apply WF.
+    - apply sub_alist_add'; auto.
+      eapply is_fresh_alist_fresh; eauto.
+    - solve_fresh.
+  Qed.
+
+  Lemma state_invariant_memory_invariant' :
+    forall σ s1 s2 s li mH mV l g,
+      state_invariant'' σ s1 s2 s li mH (mV,(l,g)) ->
+      memory_invariant σ s mH (mV,(li,g)).
+  Proof.
+    intros * H; inv H; auto.
+  Qed.
+  Hint Resolve state_invariant_memory_invariant' : core.
+
+  Lemma state_invariant_sub_alist' :
+    forall σ s1 s2 s li mH mV l g,
+      state_invariant'' σ s1 s2 s li mH (mV,(l,g)) ->
+      li ⊑ l.
+  Proof.
+    intros * H; inv H; auto.
+  Qed.
+  Hint Resolve state_invariant_sub_alist' : core.
+
+  Definition ext_local {R S} (e : exp typ) : config_helix -> config_cfg -> Rel_cfg_T R S :=
+    fun mh '(mi,(li,gi)) '(mh',_) '(m,(l,(g,_))) =>
+      mh ≡ mh' /\ mi ≡ m /\ gi ≡ g.
+      (* /\ (forall id, e ≡ EXP_Ident (ID_Local id) -> alist_find id l ≡ alist_find id li). *)
+      (* (s1 ≡ s2 \/ exists s id, incLocal s ≡ inr (s2,id) /\ alist_find id l ≡ alist_find id li). *)
+      (* (forall id v, *)
+      (*   alist_In id l v -> *)
+      (*   ~ alist_In id li v -> *)
+      (*   lid_bound_between s1 s2 id). *)
+
+  Definition genNExpr_exp_correct (e: exp typ) (* (li : local_env) *)
+  : Rel_cfg_T DynamicValues.int64 unit :=
+    fun '(x,i) '(memV,(l,(g,v))) =>
+      forall l',
+        (* li ⊑ l' -> *)
+        (forall id, e ≡ EXP_Ident (ID_Local id) -> alist_find id l' ≡ alist_find id l)
+        ->
+        interp_cfg
+          (translate exp_E_to_instr_E (denote_exp (Some (DTYPE_I 64%Z)) (convert_typ [] e)))
+          g l' memV ≈
+          Ret (memV,(l',(g,UVALUE_I64 i))).
+
+  Lemma incLocal_ineq: forall s1 s2 r,
+      incLocal s1 ≡ inr (s2,r) -> s1 <> s2.
+  Proof.
+    intros.
+    Transparent incLocal.
+    cbn in *; inv H.
+    Opaque incLocal.
+    destruct s1; cbn.
+    intros EQ; inv EQ.
+    eapply Nat.neq_succ_diag_r; eauto.
+  Qed.
+
+  Lemma state_invariant_sub_alist_alist_add: forall s1 s2 s r σ li memH memV l g v,
+      incLocal s1 ≡ inr (s2,r) ->
+      state_invariant'' σ s1 s2 s li memH (memV, (l,g)) ->
+      li ⊑ alist_add r v l.
+  Proof.
+    intros * INC PRE; inv PRE.
+    apply sub_alist_add'; auto.
+    eapply is_fresh_alist_fresh; eauto.
+  Qed.
+
+  Definition local_scoped_modif (s1 s2 : IRState) (l1 : local_env) : local_env -> Prop :=
+    fun l2 =>
+      forall id,
+        alist_find id l2 <> alist_find id l1 ->
+        lid_bound_between s1 s2 id.
+
+  (**
+     We package the local specific invariants. Additionally to the evaluation of the resulting expression,
+     we also state that evaluating the code preserves most of the state, except for the local state being
+     allowed to be extended with fresh bindings.
+   *)
+  Record genNExpr_post
+         (e : exp typ)
+         (li : local_env)
+         s1 s2
+         (mi : memoryH) (sti : config_cfg)
+         (mf : memoryH * DynamicValues.int64) (stf : config_cfg_T unit)
+    : Prop :=
+    {
+    exp_correct' : genNExpr_exp_correct e (* li *) mf stf;
+    almost_pure : ext_local e mi sti mf stf; 
+    extends : local_scoped_modif s1 s2 (fst (snd sti)) (fst (snd stf));
+    exp_in_scope : forall id, e ≡ EXP_Ident (ID_Local id) ->
+                         ((exists v, alist_In id li v) \/ (lid_bound_between s1 s2 id /\ s1 << s2));
+    ext_li : li ⊑ (fst (snd stf))
+    }.
+
+  Set Nested Proofs Allowed.
+  Lemma local_scoped_modif_refl: forall s1 s2 l, local_scoped_modif s1 s2 l l.
+  Admitted.
+  Hint Resolve local_scoped_modif_refl: core.
+
+  Lemma local_scoped_modif_add: forall s1 s2 l r v,
+      lid_bound_between s1 s2 r ->   
+      local_scoped_modif s1 s2 l (alist_add r v l).
+  Admitted.
+
+  Lemma sub_alist_alist_find_in :
+    forall (l2 l1 : local_env) id v,
+      alist_In id l1 v ->
+      l1 ⊑ l2 ->
+      l2 @ id ≡ l1 @ id.
+  Admitted.
+
+  Lemma alist_find_eq_dec : 
+    forall {K V : Type} {RD:RelDec (@Logic.eq K)} {RDC:RelDec_Correct RD}
+      k (m1 m2 : alist K V),
+      {m2 @ k ≡ m1 @ k} + {m2 @ k <> m1 @ k}.
+  Admitted.
+
+  Lemma local_scoped_modif_out:
+    forall (l1 l2 : local_env) id s1 s2 s3,
+      s1 << s2 ->
+      lid_bound_between s1 s2 id ->
+      local_scoped_modif s2 s3 l1 l2 ->
+      l2 @ id ≡ l1 @ id.
+  Proof.
+    intros * LT BOUND SCOPE.
+    red in SCOPE.
+    edestruct @alist_find_eq_dec as [EQ | NEQ]; [| eassumption |]; [typeclasses eauto |].
+    exfalso; apply SCOPE in NEQ; clear SCOPE.
+    (* should be true *)
+  Admitted.
+
+
+  Lemma genNExpr_correct :
     forall (* Compiler bits *) (s1 s2: IRState)
       (* Helix  bits *)   (nexp: NExpr) (σ: evalContext) (memH: memoryH) 
-      (* Vellvm bits *)   (e: exp typ) (c: code typ) (g : global_env) (l : local_env) (memV : memoryV),
+      (* Vellvm bits *)   (e: exp typ) (c: code typ) (g : global_env) (li l : local_env) (memV : memoryV),
 
       genNExpr nexp s1 ≡ inr (s2, (e, c))      -> (* Compilation succeeds *)
-      (state_invariant_pre σ s1 s2) memH (memV, (l, g)) -> (* The main state invariant is initially true *)
+      (state_invariant'' σ s1 s2 s1 li) memH (memV, (l, g)) -> (* The main state invariant is initially true *)
       no_failure (interp_helix (E := E_cfg) (denoteNExpr σ nexp) memH) -> (* Source semantics defined *)
-      eutt (succ_cfg (lift_Rel_cfg (state_invariant_post σ s1 s2 l) ⩕
-                     genNExpr_rel_ind e memH (mk_config_cfg memV l g)))
+      eutt (succ_cfg (lift_Rel_cfg (state_invariant'' σ s1 s2 s2 li) ⩕
+                     genNExpr_post e li s1 s2 memH (mk_config_cfg memV l g)))
            (interp_helix (denoteNExpr σ nexp) memH)
            (interp_cfg (denote_code (convert_typ [] c)) g l memV).
   Proof.
-    intros s1 s2 nexp; revert s1 s2; induction nexp; intros * COMPILE [PRE PREF] NOFAIL.
-
+    intros s1 s2 nexp; revert s1 s2; induction nexp; intros * COMPILE PRE NOFAIL.
     - (* Variable case *)
       (* Reducing the successful compilation *)
       cbn* in COMPILE; simp.
@@ -121,50 +365,86 @@ Section NExpr.
         hvred.
 
         (* The identifier has to be a local one *)
-        destruct i0; try_abs.
+        destruct i0.
+        inv PRE; try_abs.
 
         (* We establish the postcondition *)
-        apply eutt_Ret; cbn; split_post. 
-        intros l' MONO; cbn*.
-        vstep.
-        solve_lu.
-        reflexivity.
+        apply eutt_Ret; split; [| split]; cbn; eauto.
+        * intros l' VAR; cbn*.
+          inv PRE.
+          vstep.
+          cbn.
+          rewrite VAR; auto.
+          eapply memory_invariant_LLU; eauto.
+          reflexivity.
+        * intros * EQ; inv EQ.
+          left.
+          eexists.
+          eapply memory_invariant_LLU; eauto.
 
       + (* The variable maps to a pointer *)
         unfold denoteNExpr in *; cbn* in *; simp; try_abs.
         break_inner_match_goal; try_abs.
+        2:inv PRE; try_abs.
+ 
         hvred.
         (* We need to be a bit careful: when stepping the [load], we will need to provide the memory address
            at which we load. This address needs to be in scope when introducing the evar, we are therefore
            forced to look a bit ahead and first use [memory_invariant_GLU].
          *)
+
         edestruct memory_invariant_GLU as (ptr & LU & READ); eauto.
+
         rewrite typ_to_dtyp_equation in READ.
         vstep.
         vstep; eauto; reflexivity.
+        apply eutt_Ret; cbn; split; [| split]; cbn; eauto.
+        * apply state_invariant_add_fresh''; auto.
+        * intros l' VAR; cbn*.
+          vstep; [ | reflexivity].
+          cbn; erewrite VAR; eauto.
+          rewrite eq_dec_eq; reflexivity.
+        * apply local_scoped_modif_add.
+          auto using lid_bound_between_incLocal.
+        * intros * EQ; inv EQ; right.
+          split; [auto using lid_bound_between_incLocal | solve_local_count].
+        * eapply state_invariant_sub_alist_alist_add; eauto.
+        (* eapply incLocal_ineq; eauto. *)
 
-        apply eutt_Ret; cbn; split_post.
-        intros l' MONO; cbn*.
-        vstep; [solve_lu | reflexivity].
-        repeat split.
-        solve_sub_alist.
+        (* * intuition. *)
+        (*   inv H. *)
+        (*   rewrite eq_dec_eq. *)
+
+        (*   rename r into foo. *)
+        (*   right; do 2 eexists; split; eauto. *)
+        (*   rewrite eq_dec_eq. rename r into foo. *)
+        (*   symmetry. *)
+
+        (*   eauto. *)
+          (* destruct (id0 ?[ Logic.eq ] r) eqn:EQ. *)
+          (* rewrite rel_dec_correct in EQ; subst; auto using lid_bound_between_incLocal. *)
+          (* apply neg_rel_dec_correct in EQ. *)
+          (* apply In_add_In_ineq in H; intuition. *)
 
     - (* Constant *)
       cbn* in COMPILE; simp.
       unfold denoteNExpr in *; cbn*.
       hvred.
 
-      apply eutt_Ret; cbn; split_post. 
+      apply eutt_Ret; split; [| split]; cbn; eauto.
       intros l' MONO; cbn*.
       vstep; reflexivity.
+      intros * EQ; inv EQ.
 
     - (* NDiv *)
       cbn* in *; simp; try_abs.
       hvred.
+      rename i into s2, i0 into s3, s2 into s4.
+      clean_goal.
 
-      specialize (IHnexp1 _ _ σ memH _ _ g l memV Heqs).
+      specialize (IHnexp1 _ _ σ memH _ _ g li l memV Heqs).
       forward IHnexp1.
-      { split; auto.
+      { inv PRE; split; auto.
         solve_fresh.
       }
       forward IHnexp1; eauto.
@@ -173,54 +453,79 @@ Section NExpr.
       eapply eutt_clo_bind_returns ; [eassumption | clear IHnexp1].
       introR; destruct_unit.
       intros RET _; eapply no_failure_helix_bind_continuation in NOFAIL; [| eassumption]; clear RET.
-      destruct PRE0 as ((PRE1 & PREF1) & (EXPR1 & <- & <- & <- & MONO1)). 
+      destruct PRE0 as (PRE1 & [EXP1 EXT1 SCOPE1 VAR1 EXTI1]).
+      cbn* in *; inv_eqs.
+      (* rename H into VAR1. *)
       hvred.
-      cbn in *.
 
       (* e2 *)
-      specialize (IHnexp2 _ _ σ memH _ _ g l0 memV Heqs0).
+      specialize (IHnexp2 _ _ σ memH _ _ g li l0 memV Heqs0).
       forward IHnexp2.
       {
-        split; auto.
-        solve_fresh.
+        clean_goal.
+        inv PRE; inv PRE1.
+        constructor; auto.
+        eapply is_fresh_shrink with (1 := FRESH). 
+        solve_local_count.
+        solve_local_count.
       }
       forward IHnexp2; eauto.
 
       eapply eutt_clo_bind_returns ; [eassumption | clear IHnexp2].
       introR; destruct_unit.
       intros RET _; eapply no_failure_helix_bind_continuation in NOFAIL; [| eassumption]; clear RET.
-      destruct PRE0 as ((PRE2 & PREF2) & (EXPR2 & <- & <- & <- & MONO2)).
-      cbn in *.
+      destruct PRE0 as (PRE2 & [EXP2 EXT2 SCOPE2 VAR2 EXTI2]).
+      cbn* in *; inv_eqs.
+      (* rename H into VAR2. *)
 
       (* division *)
       simp; try_abs.
       hvred.
 
-      specialize (EXPR1 _ MONO2) .
-      assert (l1 ⊑ l1) as L1L1 by reflexivity; specialize (EXPR2 _ L1L1). 
-      cbn in *.
+      specialize (EXP1 l1) .
+      specialize (EXP2 l1) .
+      forward EXP2; [intros; reflexivity |].
+      forward EXP1.
+      {
+        clear EXP1 EXP2.
+        clean_goal.
+        intros * EQE.
+        apply VAR1 in EQE.
+        destruct EQE as [[?v IN] | [BOUND LT]].
+        erewrite sub_alist_alist_find_in; [| eauto | eauto].
+        erewrite (@sub_alist_alist_find_in l0); [| eauto | eauto]; reflexivity.
+        clear n Heqd NOFAIL VAR1 VAR2.
+        eapply local_scoped_modif_out; eauto.
+      }
+
       hvred.
       vstep.
       {
         vstep; eauto; try reflexivity.
         cbn; break_inner_match_goal; try reflexivity.
         exfalso; apply n.
-        clear EXPR2 EXPR1.
         apply Z.eqb_eq in Heqb.
         rewrite <- Int64.unsigned_zero in Heqb.
         unfold MInt64asNT.NTypeZero.
         apply unsigned_is_zero; auto.
       }
 
-      apply eutt_Ret; cbn; split_post.
-      intros ? MONO; cbn.
-      vstep; solve_lu; reflexivity.
-      etransitivity; eauto.
-      etransitivity; eauto.
-      apply sub_alist_add.
-      eapply freshness_pre_alist_fresh; eauto.
-      solve_fresh.
-  
+      apply eutt_Ret; cbn; split; [| split]; cbn; eauto.
+      + admit.
+      + intros * VAREQ.
+        specialize (VAREQ r eq_refl); rewrite eq_dec_eq in VAREQ.
+        vstep; eauto; reflexivity.
+      + admit.
+      + admit.
+      + admit.
+        (* intros ? MONO; cbn. *)
+        (* vstep; solve_lu; reflexivity. *)
+        (* etransitivity; eauto. *)
+        (* etransitivity; eauto. *)
+        (* apply sub_alist_add. *)
+        (* eapply freshness_pre_alist_fresh; eauto. *)
+        (* solve_fresh. *)
+        
     - (* NMod *)
       cbn* in *; simp; try_abs.
       hvred.
